theories/partial/choice/pmatch.v
@@ -58,3 +58,62 @@ Proof.
     assumption.
 Qed.
     
+Definition Pmatch2 {T1 T2 A : Type} (P : T1 -> T2 -> Prop)
+           (branch1 : T1 -> T2 -> A) (branch2 : A) : A.
+  refine (choose A (fun a => (exists t1 t2, P t1 t2 /\ branch1 t1 t2 = a)
+                             \/
+                               ((~exists t1 t2, P t1 t2) /\ a = branch2))).
+  destruct (classic (exists t1 t2, P t1 t2)).
+  - destruct H, H.
+    exists (branch1 x x0).
+    apply or_introl.
+    exists x.
+    exists x0.
+    auto.
+  - exists branch2.
+    apply or_intror.
+    split; auto.
+Defined.
+
+Theorem Pmatch2Def1 {T1 T2 A : Type} {P : T1 -> T2 -> Prop} {t1 : T1} {t2 : T2} (H : P t1 t2)
+        (*(unique : forall t1 t2 t1' t2', P t1 t2 -> P t1' t2' -> t1 = t1' /\ t2 = t2')*)
+        (unique1 : forall t1 t2 t1' t2', P t1 t2 -> P t1' t2' -> t1 = t1')
+        (unique2 : forall t1 t2 t1' t2', P t1 t2 -> P t1' t2' -> t2 = t2')
+        (branch1 : T1 -> T2 -> A) (branch2 : A)
+  : Pmatch2 P branch1 branch2 = branch1 t1 t2.
+Proof.
+  unfold Pmatch2.
+  apply choiceInd.
+  intros.
+  destruct H0.
+  - destruct H0, H0, H0.
+    specialize (unique1 _ _ _ _ H H0).
+    specialize (unique2 _ _ _ _ H H0).
+    subst.
+    reflexivity.
+  - destruct H0.
+    exfalso.
+    apply H0.
+    exists t1.
+    exists t2.
+    assumption.
+Qed.
+
+Theorem Pmatch2Def2 {T1 T2 A : Type} (P : T1 -> T2 -> Prop)
+        (*unique : forall t1 t2, P t1 -> P t2 -> t1 = t2*)
+        (branch1 : T1 -> T2 -> A) (branch2 : A)
+        (ne : forall t1 t2, P t1 t2 -> False)
+  : Pmatch2 P branch1 branch2 = branch2.
+Proof.
+  unfold Pmatch2.
+  apply choiceInd.
+  intros.
+  destruct H.
+  - destruct H, H, H.
+    exfalso.
+    apply (ne x x0).
+    assumption.
+  - destruct H.
+    assumption.
+Qed.
+    
