theories/embeddingMetaprogramTest.v
@@ -1,0 +1,355 @@
+Require Import String.
+Require Import qterm.
+Require Import lambdaFacts.
+Require Import lambdaSolve.
+Require Import FunctionalExtensionality.
+Require Import Coq.Logic.PropExtensionality.
+
+Definition nil := <Nil>.
+Definition cons := <fun ctx => fun lvl => fun ty => Cons ctx lvl ty>.
+
+Definition zero := <fun env => proj2 env>.
+Definition succ := <fun x => fun env => x (proj1 env)>.
+
+Definition level (n : nat) : QTerm := const n.
+(* Should I have an explicit type level on the pis? *)
+Definition pi := <fun x => fun y => fun env => Pi (x env) (fun a => y (env , a))>.
+Definition U : QTerm := <(*fun lvl => *)fun env => U (*lvl*)>.
+Definition Empty := <fun env => Empty>.
+Definition Bool := <fun env => Bool>.
+Definition Lift := <fun T => fun env => Lift (T env)>.
+
+Definition var_to_term := <fun x => x>.
+Definition lambda := <fun t => fun env => fun a => t (env , a)>.
+Definition app := <fun t1 => fun t2 => fun env => (t1 env) (t2 env)>.
+Definition true := <fun env => fun p => proj1 p>.
+Definition false := <fun env => fun p => proj2 p>.
+Definition ifexpr := <fun cond => fun t1 => fun t2 => fun env => (cond env) (t1 env, t2 env)>.
+
+Definition weaken := <fun t => fun env => t (proj1 env)>.
+Definition subLast := <fun t => fun toSub => fun env => t (env , toSub env)>.
+
+Ltac unfold_all := unfold nil, cons, zero, succ, pi, U, Bool, Empty, var_to_term, lambda,
+    app, weaken, subLast, level, true, false, ifexpr, Lift in *.
+
+(* The deeper shallow embedding *)
+
+Inductive VarTyped : QTerm -> nat -> QTerm -> QTerm -> Prop :=
+| ty_zero : forall ctx T lvl, VarTyped <`cons `ctx {const lvl} `T> lvl <`weaken `T> zero
+| ty_succ : forall ctx A T s lvl1 lvl2, VarTyped ctx lvl1 A s
+                              -> VarTyped <`cons `ctx `lvl2 `T> lvl1 <`weaken `A> <`succ `s>.
+
+Inductive Typed : (*context*) QTerm -> (*level*) nat -> (*Type*) QTerm -> (*Term*) QTerm -> Type :=
+| ty_lambda : forall {ctx A B s lvl},
+    (*Typed ctx (S lvl) <`U(*{const lvl}*)> <`pi `A `B> ->*)
+    Typed <`cons `ctx {const lvl} `A> lvl B s -> Typed ctx lvl <`pi `A `B> <`lambda `s>
+(*
+| ty_app : forall ctx A B s1 s2 lvl, Typed ctx lvl <`pi `A `B> s1 -> Typed ctx lvl A s2
+                                 -> Typed ctx lvl <`subLast `B `s2> <`app `s1 `s2>
+| ty_var : forall ctx T t lvl, VarTyped ctx lvl T t -> Typed ctx lvl T t
+*)
+| ty_true : forall {ctx}, Typed ctx 0 Bool true
+| ty_false : forall {ctx}, Typed ctx 0 Bool false
+(*
+| ty_if : forall ctx T cond t1 t2 lvl,
+    Typed ctx lvl Bool cond ->
+    Typed ctx lvl <`subLast `T `true> t1 ->
+    Typed ctx lvl <`subLast `T `false> t2 ->
+    Typed ctx lvl <`subLast `T `cond> <`ifexpr `cond `t1 `t2>
+| ty_Empty : forall ctx, Typed ctx 1 <`U(*{const 0}*)> Empty
+| ty_Bool : forall ctx, Typed ctx 1 <`U(*{const 0}*)> Bool
+| ty_pi : forall ctx A B lvl,
+    Typed ctx (S lvl) <`U(*{const lvl}*)> A
+    (* TODO: is S lvl correct below? *)
+    -> Typed <`cons `ctx {const lvl} `A> (S lvl) <`U(*{const lvl}*)> B -> Typed ctx (S lvl) <`U(*{const lvl}*)> <`pi `A `B>
+| ty_U : forall ctx lvl, Typed ctx (S (S lvl)) <`U(*{const (S lvl)}*)> <`U(*{const lvl}*)>
+| ty_Lift : forall ctx lvl T, Typed ctx (S lvl) <`U> T -> Typed ctx (S (S lvl)) <`U> <`Lift `T>
+| ty_lift : forall ctx lvl T t, Typed ctx lvl T t -> Typed ctx (S lvl) <`Lift `T> t
+| ty_lower : forall ctx lvl T t, Typed ctx (S lvl) <`Lift `T> t -> Typed ctx lvl T t
+*)
+.
+
+Ltac solve_no_unfold := repeat (lambda_solve ; repeat neutral_inj_case ;lambda_solve
+                  ; repeat fast_neutral_unequal_case). 
+
+Ltac solve_all := repeat (unfold_all ; lambda_solve ; repeat neutral_inj_case ;lambda_solve
+                          ; repeat fast_neutral_unequal_case).
+
+From Equations.Prop Require Import Equations.
+
+(*
+Definition defer_cast {ctx ty1 ty2 t1 t2 : QTerm} {lvl} {pty : ty1 = ty2} {pt : t1 = t2}
+  (prog : Typed ctx lvl ty1 t1) : Typed ctx lvl ty2 t2.
+  subst.
+  apply prog.
+Defined.
+ *)
+Definition defer_cast {A B : Type} {p : A = B} (a : A) : B.
+  subst.
+  apply a.
+Defined.
+
+Equations silly_transform_eq {ctx T t : QTerm} {lvl : nat} (prog : Typed ctx lvl T t) : Typed ctx lvl T t :=
+silly_transform_eq ty_true := defer_cast ty_false;
+silly_transform_eq prog := prog.
+
+Next Obligation.
+Proof.
+Abort.
+(*
+Equations match_on_id {t : QTerm} (prog : Typed nil 2 <`pi `U `U> t) : {t' & Typed <`cons {const 1} `U> 2 U t'} :=
+  match_on_id (ty_lambda t') := _;
+  match_on_id ty_true := _;
+  match_on_id ty_false := _.
+*)
+Definition silly_transform {ctx T t : QTerm} {lvl : nat} (prog : Typed ctx lvl T t) : Typed ctx lvl T t.
+  refine (
+      match prog in Typed ctx lvl T t return Typed ctx lvl T t with
+      | ty_true => defer_cast ty_false
+      | t => t
+      end
+    ); try solve_all.
+Abort.
+
+(* So that actually kind of works. *)
+
+Definition match_on_id' {t : QTerm} (prog : Typed nil 2 <`pi `U `U> t) : {t' & Typed <`cons {const 1} `U> 2 U t'}.
+  (*remember <`pi `U `U> as in_type.*)
+
+  refine (
+      match prog in Typed x1 x2 x3 x4 return {t' & Typed <`cons {const 1} `U> 2 U t'} with
+      | ty_true => _
+      | ty_false => _
+      | ty_lambda t' => _
+      end
+    ).
+Abort.
+Check lift.
+Axiom fact1 : forall (t1 t2 : QTerm) s, <`t1 [`s] {var s 0}> = t2 -> t1 = <fun `s => `t2>.
+Locate "[".
+Axiom fact2 : forall (t1 t2 : QTerm) s1 s2, <`t1 [`s1] [`s2] ({var s1 0}, {var s2 0})> = t2
+                                            -> t1 = <fun p => `t2 [`s1 / proj1 p] [`s1 / proj2 p]>.
+
+Ltac solve_all_2 := repeat (subst; solve_all;
+                            match goal with
+                            | H : (qterm.app (lift ?s ?i ?t1) (var ?s ?i))
+                                  = ?t2 |- _ => apply fact1 in H
+                            | H : (qterm.app (lift ?s2 ?i2 (lift ?s1 ?i1 ?t1))
+                                       (pair (var ?s1 ?i1) (var ?s2 ?i2)))
+                                  = ?t2 |- _ => apply fact2 in H
+                            end).
+
+(*TODO: can prove from UIP? *)
+Axiom cast_remover : forall A (p : A = A) (a : A), @defer_cast A A p a = a.
+
+Definition match_on_id' {ctx T t: QTerm} {lvl} (prog : Typed ctx lvl T t)
+  :
+  ctx = nil
+  -> lvl = 0
+  -> T = <`pi `Bool `Bool>
+  -> {t' & Typed <`cons `nil {const 0} `Bool> 0 Bool t'}.
+  refine (
+      match prog with
+      | ty_true => _
+      | ty_false => _
+      | ty_lambda t' => fun _ _ _ => (existT _ _ (defer_cast t'))
+      end
+    ); try solve[intros; solve_all_2].
+Defined.
+
+Theorem match_on_id_works : match_on_id' (ty_lambda ty_true) eq_refl eq_refl eq_refl
+                            = existT _ _ ty_true.
+Proof.
+  (*This won't be possible*)
+  simpl.
+  rewrite cast_remover.
+  reflexivity.
+Qed.
+
+(*
+TODO: Will using SProp improve performance everywhere? All my terms have huge equality proofs in them.
+Alternatively, I could periodically rewrite equalities between x = x into refls to make them smaller.
+(recursive something something?)
+*)
+
+(*
+So, this works in this case. But it probably won't always work. I'll contrive an example.
+ *)
+
+Module Test2.
+
+Axiom I : Type.
+Axiom i1 i2 : I.
+Axiom i1i2 : i1 = i2.
+
+Inductive Fam : I -> Type :=
+| fam1 : Fam i1
+| fam2 : Fam i2.
+
+Definition cast (A B : Type) {p : A = B} (a : A) : B.
+  subst.
+  apply a.
+Defined.
+
+
+Definition famswap {i : I} (f : Fam i) : Fam i.
+  refine (
+      match f with
+      | fam1 => @cast _ _ _ fam2
+      | fam2 => @cast _ _ _ fam1
+      end
+    ).
+  rewrite i1i2.
+  reflexivity.
+  rewrite i1i2.
+  reflexivity.
+Defined.
+
+Theorem famswap_works : famswap (famswap fam1) = fam1.
+Proof.
+  simpl.
+  Fail rewrite cast_remover.
+Abort.
+
+(******)
+
+Check f_equal.
+Theorem push_cast_through
+        (I : Type)
+        (P Q : I -> Type)
+        (f : forall i, P i -> Q i)
+        (i1 i2 : I)
+        (p : i1 = i2)
+        (input : P i1)
+  : f _ (@cast _ _ (f_equal P p) input) = @cast _ _ (f_equal Q p) (f _ input).
+Proof.
+  refine (match p with
+          | eq_refl => _
+          end).
+  reflexivity.
+Qed.
+
+(*
+Can I use UIP or SProp somehow to make this work better?
+
+IDEA: Use a specialized version of cast where the equality is always over the index type.
+so cast : ctx1 = ctx2 -> T1 = T2 -> t1 = t2 -> Typed ctx1 T1 t1 -> Typed ctx2 T2 t2
+sort of thing.
+
+
+*)
+
+Axiom uip : forall (T : Type) (t : T) (p : t = t), p = eq_refl.
+Theorem really_push_it_through_with_uip
+        (I : Type)
+        (P Q : I -> Type)
+        (f : forall i, P i -> Q i)
+        (i1 i2 : I)
+        (pi : i1 = i2)
+        (p2 : P i1 = P i2)
+        (input : P i1)
+  : f _ (@cast _ _ p2 input) = @cast _ _ (f_equal Q pi) (f _ input).
+Abort.
+
+Theorem famswap_works_2 : famswap (famswap fam1) = fam1.
+Proof.
+  simpl.
+  Set Printing Implicit.
+  Fail rewrite (@push_cast_through I Fam Fam (@famswap) i2 i1
+               (@eq_ind_r I i2 (fun i : I => Fam i2 = Fam i) (@eq_refl Set (Fam i2)) i1 i1i2)
+               fam2).
+Abort.
+  
+End Test2.
+
+Module Test3.
+
+Axiom I : Type.
+Axiom i1 i2 : I.
+Axiom i1i2 : i1 = i2.
+
+Inductive Fam : I -> Type :=
+| fam1 : Fam i1
+| fam2 : Fam i2.
+
+Definition transport {T : Type} (P : T -> Type) {t1 t2 : T} (p : t1 = t2) (a : P t1) : P t2.
+  subst.
+  apply a.
+Defined.
+
+Definition famswap {i : I} (f : Fam i) : Fam i.
+  refine (
+      match f with
+      | fam1 => transport Fam _ fam2
+      | fam2 => transport Fam _ fam1
+      end
+    ).
+  rewrite i1i2.
+  reflexivity.
+  rewrite i1i2.
+  reflexivity.
+Defined.
+
+Theorem famswap_works : famswap (famswap fam1) = fam1.
+Proof.
+  simpl.
+  Fail rewrite cast_remover.
+Abort.
+
+(******)
+
+Check f_equal.
+Theorem push_transport_through
+        (I : Type)
+        (P Q : I -> Type)
+        (f : forall i, P i -> Q i)
+        (i1 i2 : I)
+        (p : i1 = i2)
+        (input : P i1)
+  : f _ (transport P p input) = transport Q p (f _ input).
+Proof.
+  refine (match p with
+          | eq_refl => _
+          end).
+  reflexivity.
+Qed.
+
+Theorem compose_transport
+        (I : Type)
+        (P : I -> Type)
+        (i1 i2 i3 : I)
+        (p : i1 = i2)
+        (q : i2 = i3)
+        (input : P i1)
+  : transport P q (transport P p input) = transport P (eq_trans p q) input.
+Proof.
+  subst.
+  reflexivity.
+Qed.
+Print UIP.
+Axiom uip : forall T, UIP T.
+Theorem remove_transport
+        (I : Type)
+        (P : I -> Type)
+        (i : I)
+        (loop : i = i)
+        (input : P i)
+        : transport P loop input = input.
+Proof.
+  rewrite (uip I i i loop eq_refl).
+  reflexivity.
+Qed.
+
+Ltac escape_transport_hell :=
+  repeat (rewrite ?push_transport_through, ?compose_transport, ?remove_transport).
+  
+Theorem famswap_works_2 : famswap (famswap fam1) = fam1.
+Proof.
+  simpl.
+  escape_transport_hell.
+  simpl.
+  escape_transport_hell.
+  reflexivity.
+Qed.
+  
+End Test3.
