theories/partial/choice/automation.v
@@ -2,12 +2,20 @@ Require Import choiceBase.
 Require Import prog2.
 Require Import pmatch.
 
+Check PmatchDef1.
+Check Pmatch2Def1.
+Check PmatchDef2.
+Check Pmatch2Def2.
+
 Ltac evaluate_function solve_tactic :=
   repeat (
       unfold runProg;
       rewrite ?runProgDefinitionRet, ?runProgDefinitionRec, ?collectOptionDef;
       try (erewrite PmatchDef1 ; [| solve [solve_tactic] | solve [intros; solve_tactic]]);
       try (erewrite PmatchDef2 ; [|intros; solve [solve_tactic]]);
+      try (erewrite Pmatch2Def1 ; [| solve [solve_tactic]
+                                  | solve [intros; solve_tactic] | solve [intros; solve_tactic]]);
+      try (erewrite Pmatch2Def2 ; [|intros; solve [solve_tactic]]);
       try (erewrite PifDef1 ; [| solve [solve_tactic]]);
       try (erewrite PifDef2 ; [| intros; solve [solve_tactic]]);
       simpl
@@ -19,6 +27,9 @@ Ltac evaluate_function_in solve_tactic H :=
       rewrite ?runProgDefinitionRet, ?runProgDefinitionRec, ?collectOptionDef in H;
       try (erewrite PmatchDef1 in H ; [| solve [solve_tactic] | solve [intros; solve_tactic]]);
       try (erewrite PmatchDef2 in H ; [|intros; solve [solve_tactic]]);
+      try (erewrite Pmatch2Def1 in H ; [| solve [solve_tactic]
+                                       | solve [intros; solve_tactic] | solve [intros; solve_tactic]]);
+      try (erewrite Pmatch2Def2 in H ; [|intros; solve [solve_tactic]]);
       try (erewrite PifDef1 in H ; [| solve [solve_tactic]]);
       try (erewrite PifDef2 in H ; [| intros; solve [solve_tactic]]);
       simpl in H
